Phi_System/IDE_CP_Reasoning1.thy
@@ -114,47 +114,47 @@ ML \<open>
 structure Assertion_SS = Simpset (
   val initial_ss = Simpset_Configure.Minimal_SS
   val binding = \<^binding>\<open>assertion_simps\<close>
-  val comment_attrib = "Simplification rules normalizing an assertion. \
+  val comment = "Simplification rules normalizing an assertion. \
                        \It is applied before ToSA process."
 )
 
 structure Assertion_SS_Source = Simpset (
   val initial_ss = Simpset_Configure.Empty_SS
   val binding = \<^binding>\<open>assertion_simps_source\<close>
-  val comment_attrib = "Simp rules normalizing particularly source part of an assertion."
+  val comment = "Simp rules normalizing particularly source part of an assertion."
 )
 
 structure Assertion_SS_Target = Simpset (
   val initial_ss = Simpset_Configure.Empty_SS
   val binding = \<^binding>\<open>assertion_simps_target\<close>
-  val comment_attrib = "Simp rules normalizing particularly target part of an assertion."
+  val comment = "Simp rules normalizing particularly target part of an assertion."
 )
 
 structure Assertion_SS_Abnormal = Simpset (
   val initial_ss = Simpset_Configure.Empty_SS
   val binding = \<^binding>\<open>assertion_simps_abnormal\<close>
-  val comment_attrib = "Simp rules normalizing particularly the abnormal spec of a triple."
+  val comment = "Simp rules normalizing particularly the abnormal spec of a triple."
 )
 \<close>
 
 \<phi>reasoner_ML assertion_simp_source 1300
   (\<open>Simplify (assertion_simps SOURCE) ?X' ?X\<close>)
-  = \<open>PLPR_Simplifier.simplifier_by_ss' (fn ctxt =>
+  = \<open>PLPR_Simplifier.simplifier_by_ss' NONE (fn ctxt =>
       Raw_Simplifier.merge_ss (Assertion_SS.get' ctxt, Assertion_SS_Source.get' ctxt))\<close>
 
 \<phi>reasoner_ML assertion_simp_target 1300
   (\<open>Simplify (assertion_simps TARGET) ?X' ?X\<close>)
-  = \<open>PLPR_Simplifier.simplifier_by_ss' (fn ctxt =>
+  = \<open>PLPR_Simplifier.simplifier_by_ss' NONE (fn ctxt =>
       Raw_Simplifier.merge_ss (Assertion_SS.get' ctxt, Assertion_SS_Target.get' ctxt))\<close>
 
 \<phi>reasoner_ML assertion_simp_abnormal 1300
   (\<open>Simplify (assertion_simps ABNORMAL) ?X' ?X\<close>)
-  = \<open>PLPR_Simplifier.simplifier_by_ss' (fn ctxt =>
+  = \<open>PLPR_Simplifier.simplifier_by_ss' NONE (fn ctxt =>
       Raw_Simplifier.merge_ss (Assertion_SS.get' ctxt, Assertion_SS_Abnormal.get' ctxt))\<close>
 
 \<phi>reasoner_ML assertion_simp 1300
   (\<open>Simplify (assertion_simps ?ANY) ?X' ?X\<close>)
-  = \<open>PLPR_Simplifier.simplifier_by_ss' Assertion_SS.get'\<close>
+  = \<open>PLPR_Simplifier.simplifier_by_ss' NONE Assertion_SS.get'\<close>
 
 lemmas [assertion_simps] =
   mult_zero_right[where 'a=\<open>'a::sep_magma set\<close>] mult_zero_left[where 'a=\<open>'a::sep_magma set\<close>]
@@ -342,7 +342,7 @@ declare mult.assoc[symmetric, frame_var_rewrs]
 consts frame_var_rewrs :: mode
 
 \<phi>reasoner_ML Subty_Simplify 2000 (\<open>Simplify frame_var_rewrs ?x ?y\<close>)
-  = \<open>PLPR_Simplifier.simplifier_only (fn ctxt =>
+  = \<open>PLPR_Simplifier.simplifier_only NONE (fn ctxt =>
           Named_Theorems.get ctxt \<^named_theorems>\<open>frame_var_rewrs\<close>)\<close>
 
 definition \<phi>IntroFrameVar :: "'a::sep_magma_1 set \<Rightarrow> 'a set \<Rightarrow> 'a set \<Rightarrow> 'a set \<Rightarrow> 'a set \<Rightarrow> bool"
